@@ -9,4 +9,7 @@ namespace Xv6
 theorem Acquiresleep (AC : ACQUIRE) (RE : RELEASE) (MP : MYPROC) (SP : SLEEP_PREPARE)
     (SL : SLEEP) : ACQUIRESLEEP := acquiresleep_proof AC RE MP SP SL
 
+theorem AcquiresleepNb (AC : ACQUIRE) (RE : RELEASE) (MP : MYPROC) : ACQUIRESLEEP_NB :=
+  acquiresleep_nb_proof AC RE MP
+
 end Xv6
